dfy/Map.dfy
@@ -1,0 +1,73 @@
+module Map {
+    import opened Seq
+    
+    ghost function map_sum_spec<T>(m: map<T,int>) : (sum: int)
+        ensures Seq.seq_sum(map_vals_to_seq_spec(m)) == sum
+    {
+        if |m| == 0 then
+            0
+        else if |m| == 1 then
+            var x := map_pick(m);
+            m[x]
+        else
+            var x := map_pick(m);
+            m[x] + map_sum_spec(m - {x})
+    }
+
+    ghost function map_pick<K,V>(m: map<K,V>) : (x: K)
+        requires |m| != 0
+        ensures x in m && x in m.Keys && m[x] in m.Values
+    {
+        var x :| x in m; x
+    }
+
+    ghost function map_vals_to_multiset<K,V>(m: map<K,V>) : (out: multiset<V>)
+    {
+        if |m| == 0 
+        then multiset([])
+        else 
+            var k := map_pick(m);
+            multiset([m[k]]) + map_vals_to_multiset(m - {k})
+    }
+
+    ghost function map_vals_to_seq_spec<K,V>(m: map<K,V>) : (out: seq<V>)
+        ensures map_vals_to_multiset(m) == multiset(out)
+    {
+        if |m| == 0 
+        then [] 
+        else 
+            var k := map_pick(m);
+            [m[k]] + map_vals_to_seq_spec(m - {k})
+    }
+
+    method map_vals_to_seq<K,V>(m: map<K,V>) returns (out: seq<V>)
+        decreases m
+        ensures multiset(out) == multiset(map_vals_to_seq_spec(m))
+    {
+        if |m| == 0 {
+            out := [];
+        } else {
+            var x :| x in m;
+            var remaining := map_vals_to_seq(m - {x});
+            out := [m[x]] + remaining;
+        }
+    }
+
+    
+    function map_sum<T>(m: map<T,int>) : (sum: int)
+        decreases |m|
+        ensures sum == map_sum_spec(m)
+    {
+        if |m| == 0 then
+            0
+        else
+            var x := map_pick(m);
+            m[x] + map_sum_spec(m - {x})
+    }
+    by method
+    {
+        var ss := map_vals_to_seq(m);
+        DifferentPermutationSameSum(ss, map_vals_to_seq_spec(m));
+        sum := seq_sum(ss);
+    }
+}
