dfy/Util.dfy
@@ -1,0 +1,18 @@
+include "Map.dfy"
+include "Seq.dfy"
+include "Set.dfy"
+
+module Util {
+    import opened Map
+    import opened Set
+    import opened Seq
+
+function max(a: int, b: int) : (m: int)
+    ensures m >= a
+    ensures m >= b
+    ensures m == a || m == b
+{
+    if a >= b then a else b
+}
+
+}
